a shared reduction from FRACTRAN_REG_HALING to both MMA2_HALTING and MMA2_HALTS_ON_ZERO. This avoids the detour through the compiler for the reduction from MMA2_HALTING to MMA2_HALTS_ON_ZERO, hence avoids having to describe it in a paper

theories/MinskyMachines/MM.v
@@ -46,6 +46,10 @@ Inductive mm_instr (X : Set) : Set :=
 Notation INC := mm_inc.
 Notation DEC := mm_dec.
 
+Notation INCₐ := mm_inc.
+Notation DECₐ := mm_dec.
+
+
 (* ** Semantics for MM, restricted to X = pos n for some n *)
 
 Section Minsky_Machine.
@@ -68,9 +72,9 @@ Section Minsky_Machine.
   (* Minsky machine alternate small step semantics *)
 
   Inductive mma_sss : mm_instr (pos n) -> mm_state -> mm_state -> Prop :=
-    | in_mma_sss_inc   : forall i x v,                   INC x   // (i,v) -1> (1+i,v[(S (v#>x))/x])
-    | in_mma_sss_dec_0 : forall i x k v,   v#>x = O   -> DEC x k // (i,v) -1> (1+i,v)
-    | in_mma_sss_dec_1 : forall i x k v u, v#>x = S u -> DEC x k // (i,v) -1> (k,v[u/x])
+    | in_mma_sss_inc   : forall i x v,                   INCₐ x   // (i,v) -1> (1+i,v[(S (v#>x))/x])
+    | in_mma_sss_dec_0 : forall i x k v,   v#>x = O   -> DECₐ x k // (i,v) -1> (1+i,v)
+    | in_mma_sss_dec_1 : forall i x k v u, v#>x = S u -> DECₐ x k // (i,v) -1> (k,v[u/x])
   where "i // s -1> t" := (mma_sss i s t).
 
 End Minsky_Machine.
