theories/MinskyMachines/MMA/fractran_mma.v
@@ -26,10 +26,12 @@ Tactic Notation "rew" "length" := autorewrite with length_db.
 
 Local Notation "e #> x" := (vec_pos e x).
 Local Notation "e [ v / x ]" := (vec_change e x v).
+Local Notation ø := vec_nil.
 
-Local Notation "P /MM2/ s -+> t" := (sss_progress (@mma_sss _) P s t) (at level 70, no associativity).
-Local Notation "P /MM2/ s ->> t" := (sss_compute (@mma_sss _) P s t) (at level 70, no associativity).
-Local Notation "P /MM2/ s ↓" := (sss_terminates (@mma_sss _) P s) (at level 70, no associativity). 
+Local Notation "P //ₐ s -+> t" := (sss_progress (@mma_sss _) P s t) (at level 70, no associativity).
+Local Notation "P //ₐ s ->> t" := (sss_compute (@mma_sss _) P s t) (at level 70, no associativity).
+Local Notation "P //ₐ s ~~> t" := (sss_output (@mma_sss _) P s t) (at level 70, no associativity).
+Local Notation "P //ₐ s ↓" := (sss_terminates (@mma_sss _) P s) (at level 70, no associativity). 
 
 Local Notation "l /F/ x → y" := (fractran_step l x y) (at level 70, no associativity).
 
@@ -41,6 +43,17 @@ Section Fractran_with_two_counters.
   Hint Rewrite mma_null_length mma_transfert_length mma_incs_length mma_decs_copy_length 
                mma_mult_cst_length mma_decs_length mma_mod_cst_length mma_div_cst_length : length_db.
 
+  Notation JUMPₐ := mma_jump.
+  Notation NULLₐ := mma_null.
+  Notation TRANSFERTₐ := mma_transfert.
+  Notation INCSₐ := mma_incs.
+  Notation DECSₐ := mma_decs.
+  Notation DECS_COPYₐ := mma_decs_copy.
+  Notation MULT_CSTₐ := mma_mult_cst.
+  Notation MOD_CSTₐ := mma_mod_cst.
+  Notation DIV_CSTₐ := mma_div_cst.
+  Notation LOOPₐ := mma_loop.
+
   Let src : pos 2 := pos0.
   Let dst : pos 2 := pos1.
 
@@ -49,79 +62,62 @@ Section Fractran_with_two_counters.
   Let Hsrc_dst : src <> dst.    Proof. discriminate. Qed.
   Let Hdst_src : dst <> src.    Proof. discriminate. Qed.
 
-  Section mma_loop.
-
-    Definition mma_loop := INC src :: DEC src 1 :: nil.
-
-    Fact mma_loop_loop v : (1,mma_loop) /MM2/ (1,v) -+> (1,v).
-    Proof.
-      unfold mma_loop.
-      mma sss INC with src.
-      mma sss DEC S with src 1 (v#>src); rew vec.
-      mma sss stop.
-    Qed.
-
-    Theorem mma_loop_spec v : ~ (1,mma_loop) /MM2/ (1,v) ↓.
-    Proof.
-      intros (w & (k & Hk) & H2); revert w Hk H2.
-      induction on k as IHk with measure k; intros w Hk Hw.
-      destruct subcode_sss_progress_inv with (4 := mma_loop_loop v) (5 := Hk)
-        as (q & H1 & H2); auto.
-      { apply mma_sss_fun. }
-      apply IHk with (1 := H1) (2 := H2); auto.
-    Qed.
-  
-  End mma_loop.
-
   Section mma_fractran_one.
 
     (* FRACTRAN computation, try one fraction a/b *)
 
-    Variables (a b : nat) (p i : nat).
+    Variables (p q : nat) (j i0 : nat).
+
+    Notation i := i0.
+    Notation i1 := (5+p+i0).
+    Notation i2 := (11+p+4*q+i0).
+    Notation i3 := (16+p+7*q+i0).
+    Notation i4 := (21+p+7*q+i0).
+    Notation i5 := (26+4*p+7*q+i0).
 
     Definition mma_fractran_one :=
-           mma_mult_cst src dst a i
-        ++ mma_mod_cst dst src (11+a+4*b+i) (21+a+7*b+i) b (5+a+i)
-        ++ mma_div_cst src dst b (11+a+4*b+i)
-        ++ mma_transfert dst src (16+a+7*b+i)
-        ++ INC dst :: DEC dst p
-        :: mma_div_cst src dst a (21+a+7*b+i)
-        ++ mma_transfert dst src (26+4*a+7*b+i).
+           MULT_CSTₐ src dst p i0
+        ++ MOD_CSTₐ dst src i2 i4 q i1
+        ++ DIV_CSTₐ src dst q i2
+        ++ TRANSFERTₐ dst src i3
+        ++ INCₐ dst :: DECₐ dst j
+        :: DIV_CSTₐ src dst p i4
+        ++ TRANSFERTₐ dst src i5.
 
-    Fact mma_fractran_one_length : length mma_fractran_one = 29+4*a+7*b.
+    Fact mma_fractran_one_length : length mma_fractran_one = 29+4*p+7*q.
     Proof. unfold mma_fractran_one; rew length; lia. Qed.
 
-    Hypothesis (Ha : a <> 0) (Hb : b <> 0).
+    Hypothesis (Hp : p <> 0) (Hq : q <> 0).
 
-    (* If the state in src is compatible with a/b then
-       src becomes src*a/b and jump at p *)
+    (* If the state in src is compatible with p/q then
+       src becomes src*p/q and jump at j *)
 
     Fact mma_fractran_one_ok_progress k v :
-            k*b = a*(v#>src)
+            k*q = p*(v#>src)
          -> v#>dst = 0
-         -> (i,mma_fractran_one) /MM2/ (i,v) -+> (p,v[k/src]).
-    Proof using Ha Hb.
+         -> (i0,mma_fractran_one) //ₐ (i0,v) -+> (j,v[k/src]).
+    Proof using Hp Hq.
       intros H1 H2; unfold mma_fractran_one.
-      apply sss_progress_trans with (5+a+i,v[0/src][(k*b)/dst]).
-      { apply subcode_sss_progress with (P := (i,mma_mult_cst src dst a i)); auto.
+      apply sss_progress_trans with (i1,v[0/src][(k*q)/dst]).
+      { apply subcode_sss_progress with (P := (i,mma_mult_cst src dst p i)); auto.
         apply mma_mult_cst_progress; auto.
         rewrite H2, <- H1; do 2 f_equal; lia. }
-      apply sss_progress_trans with (11+a+4*b+i,v[(k*b)/src][0/dst]).
-      { apply subcode_sss_progress with (P := (5+a+i,mma_mod_cst dst src (11+a+4*b+i) (21+a+7*b+i) b (5+a+i))); auto.
+      apply sss_progress_trans with (i2,v[(k*q)/src][0/dst]).
+      { apply subcode_sss_progress with (P := (i1,mma_mod_cst dst src i2 i4 q i1)); auto.
         apply mma_mod_cst_divides_progress with k; rew vec; try lia.
         f_equal; apply vec_pos_ext; intros y; dest y dst; try lia; dest y src. }
-      apply sss_progress_trans with (16+a+7*b+i,v[0/src][k/dst]).
-      { apply subcode_sss_progress with (P := (11+a+4*b+i,mma_div_cst src dst b (11+a+4*b+i))); auto.
+      apply sss_progress_trans with (i3,v[0/src][k/dst]).
+      { apply subcode_sss_progress with (P := (i2,mma_div_cst src dst q i2)); auto.
         apply mma_div_cst_progress with k; auto; rew vec; try lia.
         f_equal; try lia.
         apply vec_pos_ext; intros y; dest y dst; try lia; dest y src. }
-      apply sss_progress_trans with (19+a+7*b+i,v[k/src][0/dst]).
-      { apply subcode_sss_progress with (P := (16+a+7*b+i,mma_transfert dst src (16+a+7*b+i))); auto.
+      apply sss_progress_trans with (19+p+7*q+i0,v[k/src][0/dst]).
+      { apply subcode_sss_progress with (P := (i3,mma_transfert dst src i3)); auto.
         apply mma_transfert_progress; auto.
         f_equal; try lia.
         apply vec_pos_ext; intros y; dest y dst; try lia; dest y src. }
       mma sss INC with dst.
-      mma sss DEC S with dst p 0; rew vec.
+      mma sss DEC S with dst j 0; rew vec.
       mma sss stop; f_equal.
       apply vec_pos_ext; intros y; dest y dst; try lia; dest y src. 
     Qed.
@@ -129,31 +125,31 @@ Section Fractran_with_two_counters.
     (* If the state in src is not compatible with a/b then jump at the end of the code *)
 
     Fact mma_fractran_one_nok_progress v :
-            ~ divides b (a*(v#>src))
+            ~ divides q (p*(v#>src))
          -> v#>dst = 0
-         -> (i,mma_fractran_one) /MM2/ (i,v) -+> (length mma_fractran_one+i,v).
-    Proof using Ha Hb.
+         -> (i0,mma_fractran_one) //ₐ (i0,v) -+> (length mma_fractran_one+i0,v).
+    Proof using Hp Hq.
       rewrite mma_fractran_one_length.
       intros H1 H2; unfold mma_fractran_one.
       rewrite divides_rem_eq in H1.
       revert H1.
-      generalize (div_rem_spec1 (a*(v#>src)) b)
-                 (div_rem_spec2 (a*(v#>src)) Hb).
-      generalize (div (a*(v#>src)) b) (rem (a*(v#>src)) b); intros x y H3 H4 H5.
-      apply sss_progress_trans with (5+a+i,v[0/src][(x*b+y)/dst]).
-      { apply subcode_sss_progress with (P := (i,mma_mult_cst src dst a i)); auto.
+      generalize (div_rem_spec1 (p*(v#>src)) q)
+                 (div_rem_spec2 (p*(v#>src)) Hq).
+      generalize (div (p*(v#>src)) q) (rem (p*(v#>src)) q); intros x y H3 H4 H5.
+      apply sss_progress_trans with (i1,v[0/src][(x*q+y)/dst]).
+      { apply subcode_sss_progress with (P := (i0,mma_mult_cst src dst p i0)); auto.
         apply mma_mult_cst_progress; auto.
         rewrite H2, <- H3; do 2 f_equal; lia. }
-      apply sss_progress_trans with (21+a+7*b+i,v[(a*(v#>src))/src][0/dst]).
-      { apply subcode_sss_progress with (P := (5+a+i,mma_mod_cst dst src (11+a+4*b+i) (21+a+7*b+i) b (5+a+i))); auto.
+      apply sss_progress_trans with (i4,v[(p*(v#>src))/src][0/dst]).
+      { apply subcode_sss_progress with (P := (i1,mma_mod_cst dst src i2 i4 q i1)); auto.
         apply mma_mod_cst_not_divides_progress with x y; rew vec; try lia.
         f_equal; apply vec_pos_ext; intros c; dest c dst; try lia; dest c src; lia. }
-      apply sss_progress_trans with (26+4*a+7*b+i,v[0/src][(v#>src)/dst]).
-      { apply subcode_sss_progress with (P := (21+a+7*b+i,mma_div_cst src dst a (21+a+7*b+i))); auto.
+      apply sss_progress_trans with (26+4*p+7*q+i0,v[0/src][(v#>src)/dst]).
+      { apply subcode_sss_progress with (P := (i4,mma_div_cst src dst p i4)); auto.
         apply mma_div_cst_progress with (v#>src); auto; rew vec; try lia; try ring.
         f_equal; try lia.
         apply vec_pos_ext; intros c; dest c dst; try lia; dest c src. }
-      apply subcode_sss_progress with (P := (26+4*a+7*b+i,mma_transfert dst src (26+4*a+7*b+i))); auto.
+      apply subcode_sss_progress with (P := (26+4*p+7*q+i0,mma_transfert dst src (26+4*p+7*q+i0))); auto.
       apply mma_transfert_progress; auto.
       f_equal; try lia.
       apply vec_pos_ext; intros c; dest c dst; try lia; dest c src. 
@@ -161,81 +157,81 @@ Section Fractran_with_two_counters.
 
   End mma_fractran_one.
 
+  Notation FRAC_ONEₐ := mma_fractran_one.
+
   Hint Rewrite mma_fractran_one_length : length_db.
+
+  Notation fractran_super_regular := (Forall (fun c => fst c <> 0 /\ snd c <> 0)).
 
   Section mma_fractran_step.
 
     (* One step of Fractran computation *)
 
-    Variable (p : nat).
+    Variable (j : nat).
 
-    Fixpoint mma_fractran_step ll i { struct ll } :=
-      match ll with
-        | nil       => nil
-        | (a,b)::ll => let P := mma_fractran_one a b p i
-                       in  P ++ mma_fractran_step ll (length P+i)
+    Fixpoint mma_fractran_step Q i { struct Q } :=
+      match Q with
+        | nil      => nil
+        | (p,q)::Q => let P := mma_fractran_one p q j i
+                      in  P ++ mma_fractran_step Q (length P+i)
       end.
 
-    Fact mma_fractran_step_success_progress ll i x y v : 
-            Forall (fun c => fst c <> 0 /\ snd c <> 0) ll
-         -> ll /F/ x → y
+    Fact mma_fractran_step_success_progress Q i x y v : 
+            fractran_super_regular Q
+         -> Q /F/ x → y
          -> v#>src = x
          -> v#>dst = 0
-         -> (i,mma_fractran_step ll i) /MM2/ (i,v) -+> (p,v[y/src]).
+         -> (i,mma_fractran_step Q i) //ₐ (i,v) -+> (j,v[y/src]).
     Proof.
       intros H1 H2; revert H2 i v H1.
-      induction 1 as [ a b ll x y H1 | a b ll x y H1 H2 IH2 ];
+      induction 1 as [ p q ll x y H1 | p q ll x y H1 H2 IH2 ];
         intros i v H3 H6 H7; rewrite Forall_cons_inv in H3; destruct H3 as ((H3 & H4) & H5); simpl in H3, H4;
         unfold mma_fractran_step; fold mma_fractran_step.
-      + apply subcode_sss_progress with (P := (i,mma_fractran_one a b p i)); auto.
+      + apply subcode_sss_progress with (P := (i,mma_fractran_one p q j i)); auto.
         apply mma_fractran_one_ok_progress; auto; rewrite H6, <- H1; ring.
-      + apply sss_progress_trans with (length (mma_fractran_one a b p i)+i,v).
-        { apply subcode_sss_progress with (P := (i,mma_fractran_one a b p i)); auto.
+      + apply sss_progress_trans with (length (mma_fractran_one p q j i)+i,v).
+        { apply subcode_sss_progress with (P := (i,mma_fractran_one p q j i)); auto.
           apply mma_fractran_one_nok_progress; auto; rewrite H6; auto. }
-        { apply subcode_sss_progress with (P := (length (mma_fractran_one a b p i)+i,
-                                                 mma_fractran_step ll (length (mma_fractran_one a b p i)+i))); auto.
-          apply subcode_right; lia. }
+        { apply subcode_sss_progress 
+            with (P := (length (mma_fractran_one p q j i)+i,
+                        mma_fractran_step ll (length (mma_fractran_one p q j i)+i))); auto. }
     Qed.
 
-    Fact mma_fractran_step_failure_compute ll i v : 
-            Forall (fun c => fst c <> 0 /\ snd c <> 0) ll
-         -> fractran_stop ll (v#>src)
+    Fact mma_fractran_step_failure_compute Q i v : 
+            fractran_super_regular Q
+         -> fractran_stop Q (v#>src)
          -> v#>dst = 0
-         -> (i,mma_fractran_step ll i) /MM2/ (i,v) ->> (length (mma_fractran_step ll i)+i,v).
+         -> (i,mma_fractran_step Q i) //ₐ (i,v) ->> (length (mma_fractran_step Q i)+i,v).
     Proof.
       intros H1 H2 H3; revert H1 i H2.
-      induction 1 as [ | (a,b) ll (Ha & Hb) Hll IH ]; intros i H4.
+      induction 1 as [ | (p,q) ll (Hp & Hq) Hll IH ]; intros i H4.
       + mma sss stop.
       + apply fractan_stop_cons_inv in H4; destruct H4 as (H4 & H5).
         unfold mma_fractran_step; fold mma_fractran_step.
-        set (P := mma_fractran_one a b p i); rew length.
+        set (P := mma_fractran_one p q j i); rew length.
         apply sss_compute_trans with (length P+i,v).
         { apply subcode_sss_compute with (P := (i,P)); auto.
           apply sss_progress_compute, mma_fractran_one_nok_progress; auto. }
         { apply subcode_sss_compute with (P := (length P+i,mma_fractran_step ll (length P + i))); auto.
-          { apply subcode_right; lia. }
-            replace (length P+length (mma_fractran_step ll (length P + i))+i)
-            with    (length (mma_fractran_step ll (length P + i)) + (length P+i)) by lia.
-            auto. }
+          replace (length P+length (mma_fractran_step ll (length P + i))+i)
+          with    (length (mma_fractran_step ll (length P + i)) + (length P+i)) by lia; auto. }
     Qed.
 
   End mma_fractran_step.
 
   Section fractran_mma.
 
-    Variables (ll : list (nat*nat)) (Hll : Forall (fun c => fst c <> 0 /\ snd c <> 0) ll).
+    Variables (Q : list (nat*nat)) (HQ : fractran_super_regular Q).
 
-    Let i := 1.
-
-    Definition fractran_mma := mma_fractran_step i ll i.
+    Definition fractran_mma := mma_fractran_step 1 Q 1.
 
     Lemma fractran_mma_sound v x w : 
                v#>dst = 0 
-            -> fractran_compute ll (v#>src) x
-            -> fractran_stop ll x 
+            -> fractran_compute Q (v#>src) x
+            -> fractran_stop Q x 
             -> w = v[x/src]
-            -> (i,fractran_mma) /MM2/ (i,v) ->> (length fractran_mma+i,w).
-    Proof using Hll.
+            -> (1,fractran_mma) //ₐ (1,v) ->> (length fractran_mma+1,w).
+    Proof using HQ.
       intros H1 (u & H2) H3 ?; subst w.
       revert v x H1 H2 H3.
       induction u as [ | u IHu ]; simpl; intros v y H1 H2 H3.
@@ -244,7 +240,7 @@ Section Fractran_with_two_counters.
         rewrite H2; auto.
       + destruct H2 as (z & H2 & H4).
         apply mma_fractran_step_success_progress 
-          with (1 := Hll) (p := i) (i := i) (v := v) in H2; auto.
+          with (1 := HQ) (j := 1) (i := 1) (v := v) in H2; auto.
         apply IHu with (v := v[z/src]) in H3; auto; rew vec.
         revert H3; rew vec; intros H3.
         apply sss_compute_trans with (2 := H3).
@@ -253,17 +249,17 @@ Section Fractran_with_two_counters.
 
     Lemma fractran_mma_complete v : 
                v#>dst = 0 
-            -> (i,fractran_mma) /MM2/ (i,v) ↓
-            -> ll /F/ (v#>src) ↓.
-    Proof using Hll.
+            -> (1,fractran_mma) //ₐ (1,v) ↓
+            -> Q /F/ (v#>src) ↓.
+    Proof using HQ.
       intros H1 ((j,w) & (u & H2) & H3); simpl fst in H3.
       revert v H1 H2.
       induction on u as IHu with measure u; intros v H1 H2.
-      destruct (fractran_step_dec ll (v#>src)) as [ (y & Hy) | H4 ].
+      destruct (fractran_step_dec Q (v#>src)) as [ (y & Hy) | H4 ].
       2: { exists (v#>src); split; auto; exists 0; simpl; auto. }
       generalize Hy; intros H4.
       apply mma_fractran_step_success_progress 
-        with (1 := Hll) (p := i) (i := i) (v := v) 
+        with (1 := HQ) (j := 1) (i := 1) (v := v) 
         in H4; auto.
       fold fractran_mma in H4.
       destruct subcode_sss_progress_inv with (4 := H4) (5 := H2)
@@ -276,47 +272,107 @@ Section Fractran_with_two_counters.
     Qed.
    
     Theorem fractran_mma_reduction x : 
-        ll /F/ x ↓ <-> (i,fractran_mma) /MM2/ (i,x##0##vec_nil) ↓.
-    Proof using Hll.
+        Q /F/ x ↓ <-> (1,fractran_mma) //ₐ (1,x##0##ø) ↓.
+    Proof using HQ.
       split; auto.
       + intros (y & H2 & H3).
-        exists (length fractran_mma+i,y##0##vec_nil); split; simpl; auto; try lia.
+        exists (length fractran_mma+1,y##0##vec_nil); split; simpl; auto; try lia.
         apply fractran_mma_sound with (x := y); auto.
       + apply fractran_mma_complete; auto.
     Qed.
 
   End fractran_mma.
 
+  Section fractran_mma0.
+
+    Variables (Q : list (nat*nat)) (HQ : fractran_super_regular Q).
+
+    Let P := fractran_mma Q.
+
+    Definition fractran_mma0 := P ++ NULLₐ src (length P + 1) ++ JUMPₐ 0 src.
+
+    Let fmma0_1 v : v#>dst = 0 -> (1,fractran_mma0) //ₐ (length P+1,v) -+> (0,0##0##ø).
+    Proof.
+      vec split v with x; vec split v with y; vec nil v; clear v; simpl; intros ->.
+      unfold fractran_mma0.
+      apply subcode_sss_progress with (P := (length P+1, NULLₐ src (length P + 1) ++ JUMPₐ 0 src)); auto.
+      apply sss_progress_trans with (length (NULLₐ src (length P + 1)) + length P+1,0##0##ø).
+      + apply subcode_sss_progress with (P := (length P+1,NULLₐ src (length P+1))); auto.
+        apply mma_null_progress; auto.
+      + apply subcode_sss_progress with (2 := mma_jump_progress _ src _ _); auto.
+    Qed.
+
+    Lemma fractran_mma0_sound v x : 
+               v#>dst = 0 
+            -> fractran_compute Q (v#>src) x
+            -> fractran_stop Q x 
+            -> (1,fractran_mma0) //ₐ (1,v) ->> (0,0##0##ø).
+    Proof using HQ.
+      intros H1 H2 H3.
+      unfold fractran_mma0.
+      apply sss_compute_trans with (length P+1,x##0##ø).
+      + apply subcode_sss_compute with (P := (1,P)); auto.
+        apply fractran_mma_sound with (3 := H2); auto.
+        unfold src; apply vec_pos_ext; intros p; repeat invert pos p; rew vec.
+      + apply sss_progress_compute, fmma0_1; auto.
+    Qed.
+
+    Variable x : nat.
+
+    Let Term1 := Q /F/ x ↓.
+    Let Term2 := (1,fractran_mma0) //ₐ (1,x##0##ø) ~~> (0,0##0##ø).
+    Let Term3 := (1,fractran_mma0) //ₐ (1,x##0##ø) ↓.
+
+    Theorem fractran_mma0_reduction : 
+         (Term1 -> Term2) /\ (Term2 -> Term3) /\ (Term3 -> Term1).
+    Proof using HQ.
+      msplit 2; unfold Term1, Term2, Term3.
+      + intros (y & H1 & H2); split; simpl; auto.
+        apply fractran_mma0_sound with (2 := H1); auto.
+      + now exists (0,0##0##ø).
+      + intros H1; apply fractran_mma_reduction; auto.
+        revert H1; apply subcode_sss_terminates.
+        unfold fractran_mma0, P; auto.
+    Qed.
+
+  End fractran_mma0.
+
 End Fractran_with_two_counters.
 
-Section fractran_mma_reg_reduction.
+Section fractran_mma_reg_reductions.
 
-  Variables (ll : list (nat*nat)).
+  Variables (Q : list (nat*nat)).
 
-  Let reduction : { P | Forall (fun c => snd c <> 0) ll -> forall x, ll /F/ x ↓ <-> (1,P) /MM2/ (1,x##0##vec_nil) ↓ }.
+  Let reduction : { P | fractran_regular Q 
+                     -> forall x, ( Q /F/ x ↓ -> (1,P) //ₐ (1,x##0##ø) ~~> (0,0##0##ø) )
+                               /\ ( (1,P) //ₐ (1,x##0##ø) ~~> (0,0##0##ø) -> (1,P) //ₐ (1,x##0##ø) ↓ )
+                               /\ ( (1,P) //ₐ (1,x##0##ø) ↓ -> Q /F/ x ↓ ) }.
   Proof.
-    destruct (Forall_Exists_dec (fun c : nat * nat => fst c <> 0)) with (l := ll) as [ H | H ].
+    destruct (Forall_Exists_dec (fun c : nat * nat => fst c <> 0)) with (l := Q) as [ H | H ].
     + intros (x,?); simpl; destruct (eq_nat_dec x 0); subst; auto. 
-    + exists (fractran_mma ll); intros Hll x.
-      apply fractran_mma_reduction.
-      revert H Hll; repeat rewrite Forall_forall; firstorder.
+    + exists (fractran_mma0 Q); intros HQ x.
+      apply fractran_mma0_reduction; red in HQ.
+      revert H HQ; repeat rewrite Forall_forall; firstorder.
     + rewrite Exists_exists in H.
-      exists mma_loop; intros Hll.
+      exists (mma_loop pos0 1); intros Hll.
       destruct H as ((x,y) & H1 & H2); simpl in H2.
       replace x with 0 in H1 by lia; clear H2.
-      intros n; split.
+      intros n; msplit 2.
       * intros H; exfalso.
         revert H; apply FRACTRAN_HALTING_zero_num.
         apply Exists_exists; exists (0,y); auto.
+      * now exists (0,0##0##ø).
       * intros H; exfalso; revert H; apply mma_loop_spec.
   Qed.
-  
+
   Definition fractran_reg_mma := proj1_sig reduction.
 
-  Theorem fractran_reg_mma_reduction : 
-                       Forall (fun c => snd c <> 0) ll 
-          -> forall x, ll /F/ x ↓ 
-                   <-> (1,fractran_reg_mma) /MM2/ (1,x##0##vec_nil) ↓.
-  Proof. apply (proj2_sig reduction). Qed.
+  Theorem fractran_reg_mma_reductions : 
+                       fractran_regular Q 
+          -> (forall x, Q /F/ x ↓ <-> (1,fractran_reg_mma) //ₐ (1,x##0##ø) ↓)
+          /\ (forall x, Q /F/ x ↓ <-> (1,fractran_reg_mma) //ₐ (1,x##0##ø) ~~> (0,(0##0##ø))).
+  Proof. 
+     do 2 (split; intros); repeat (apply (proj2_sig reduction); auto). 
+  Qed.
 
-End fractran_mma_reg_reduction.
+End fractran_mma_reg_reductions.
