theories/MinskyMachines/MMA/mma_simul.v
@@ -24,10 +24,10 @@ Tactic Notation "rew" "length" := autorewrite with length_db.
 Local Notation "e #> x" := (vec_pos e x).
 Local Notation "e [ v / x ]" := (vec_change e x v).
 
-Local Notation "P // s -+> t" := (sss_progress (@mma_sss _) P s t).
-Local Notation "P // s ->> t" := (sss_compute (@mma_sss _) P s t).
-Local Notation "P // s ~~> t" := (sss_output (@mma_sss _) P s t).
-Local Notation "P // s ↓" := (sss_terminates (@mma_sss _) P s).
+Local Notation "P //ₐ s -+> t" := (sss_progress (@mma_sss _) P s t) (at level 70, no associativity).
+Local Notation "P //ₐ s ->> t" := (sss_compute (@mma_sss _) P s t) (at level 70, no associativity).
+Local Notation "P //ₐ s ~~> t" := (sss_output (@mma_sss _) P s t) (at level 70, no associativity).
+Local Notation "P //ₐ s ↓" := (sss_terminates (@mma_sss _) P s) (at level 70, no associativity). 
 
 (* We use the generic compiler with an identity map on instructions
     to simulate termination with termination on (0,vec_zero) *)
@@ -40,8 +40,8 @@ Section mma_sim.
 
   Definition mma_instr_compile lnk (_ : nat) (ii : mm_instr (pos n)) :=
     match ii with
-      | INC k   => INC k :: nil
-      | DEC k j => DEC k (lnk j) :: nil
+      | INCₐ k   => INCₐ k :: nil
+      | DECₐ k j => DECₐ k (lnk j) :: nil
     end. 
 
   Definition mma_instr_compile_length (ii : mm_instr (pos n)) := 1.
@@ -98,22 +98,22 @@ Section mma_sim.
 
     Infix "⋈" := (@eq (vec nat n)) (at level 70, no associativity).
 
-    Local Lemma HQ1 : forall i1 v1 w1 i2 v2, v1 ⋈ w1 /\ (iP,cP) // (i1,v1) ~~> (i2,v2)     
-                    -> exists w2,    v2 ⋈ w2 /\ Q // (lnk i1,w1) ~~> (lnk i2,w2).
+    Local Lemma HQ1 : forall i1 v1 w1 i2 v2, v1 ⋈ w1 /\ (iP,cP) //ₐ (i1,v1) ~~> (i2,v2)     
+                    -> exists w2,    v2 ⋈ w2 /\ Q //ₐ (lnk i1,w1) ~~> (lnk i2,w2).
     Proof. apply (proj2_sig (projT2 lnk_Q_pair)). Qed.
 
-    Local Lemma HQ1' i1 v1 i2 v2 : (iP,cP) // (i1,v1) ~~> (i2,v2) 
-                        ->   Q // (lnk i1,v1) ~~> (lnk i2,v2).
+    Local Lemma HQ1' i1 v1 i2 v2 : (iP,cP) //ₐ (i1,v1) ~~> (i2,v2) 
+                        ->   Q //ₐ (lnk i1,v1) ~~> (lnk i2,v2).
     Proof.
       intros H; destruct (@HQ1 i1 v1 v1 i2 v2) as (w2 & <- & ?); auto.
     Qed.
 
-    Local Lemma HQ2 : forall i1 v1 w1 j2 w2, v1 ⋈ w1 /\ Q // (lnk i1,w1) ~~> (j2,w2) 
-                    -> exists i2 v2, v2 ⋈ w2 /\ (iP,cP) // (i1,v1) ~~> (i2,v2) /\ j2 = lnk i2.
+    Local Lemma HQ2 : forall i1 v1 w1 j2 w2, v1 ⋈ w1 /\ Q //ₐ (lnk i1,w1) ~~> (j2,w2) 
+                    -> exists i2 v2, v2 ⋈ w2 /\ (iP,cP) //ₐ (i1,v1) ~~> (i2,v2) /\ j2 = lnk i2.
     Proof. apply (proj2_sig (projT2 lnk_Q_pair)). Qed.
 
-    Local Lemma HQ2' i1 v1 j2 v2 :         Q // (lnk i1,v1) ~~> (j2,v2) 
-               -> exists i2, (iP,cP) // (i1,v1) ~~> (i2,v2) /\ j2 = lnk i2.
+    Local Lemma HQ2' i1 v1 j2 v2 :         Q //ₐ (lnk i1,v1) ~~> (j2,v2) 
+               -> exists i2, (iP,cP) //ₐ (i1,v1) ~~> (i2,v2) /\ j2 = lnk i2.
     Proof.
       intros H; destruct (@HQ2 i1 v1 v1 j2 v2) as (i2 & ? & <- & ? & ->); auto.
       exists i2; auto.
@@ -123,7 +123,7 @@ Section mma_sim.
  
     (* Q simulates termination of (iP,cP) while ensuring tmp1 and tmp2 stay void when it terminates *)
 
-    Local Lemma Q_spec1 : (iP,cP) // (iP,v) ↓ -> exists w', Q // (1,v) ~~> (code_end Q, w').
+    Local Lemma Q_spec1 : (iP,cP) //ₐ (iP,v) ↓ -> exists w', Q //ₐ (1,v) ~~> (code_end Q, w').
     Proof.
       intros ((i1,v1) & H1).
       exists v1.
@@ -131,7 +131,7 @@ Section mma_sim.
       destruct H1; auto.
     Qed.
 
-    Local Lemma Q_spec2 : Q // (1,v) ↓ -> (iP,cP) // (iP,v) ↓.
+    Local Lemma Q_spec2 : Q //ₐ (1,v) ↓ -> (iP,cP) //ₐ (iP,v) ↓.
     Proof.
       intros ((j,w2) & H1).
       rewrite <- (proj1 (proj2 Hlnk)) in H1.
@@ -142,8 +142,8 @@ Section mma_sim.
     Definition mma_sim := snd Q.
     Definition mma_sim_end := code_end Q.
 
-    Theorem mma_sim_spec : ((iP,cP) // (iP,v) ↓ -> exists w', (1,mma_sim) // (1,v) ~~> (1+length mma_sim, w'))
-                        /\ ((1,mma_sim) // (1,v) ↓ -> (iP,cP) // (iP,v) ↓).
+    Theorem mma_sim_spec : ((iP,cP) //ₐ (iP,v) ↓ -> exists w', (1,mma_sim) //ₐ (1,v) ~~> (1+length mma_sim, w'))
+                        /\ ((1,mma_sim) //ₐ (1,v) ↓ -> (iP,cP) //ₐ (iP,v) ↓).
     Proof.
       replace (1+length mma_sim) with (code_end Q).
       replace (1,mma_sim) with Q. 
@@ -161,7 +161,7 @@ End mma_sim.
 Section mma2_simul.
 
   (* To generalize for n register, we need a recursive nullifying code 
-     not compilcated though *)
+     not complicated though *)
 
   Variable (iP : nat) (cP : list (mm_instr (pos 2))).
 
@@ -173,7 +173,7 @@ Section mma2_simul.
   Local Definition L1 := @mma_null_length 2 pos0 eQ.
   Local Definition L2 := @mma_null_length 2 pos1 (1+eQ).
 
-  Let N_spec v : (eQ,cN) // (eQ,v) -+> (0,vec_zero).
+  Let N_spec v : (eQ,cN) //ₐ (eQ,v) -+> (0,vec_zero).
   Proof.
     unfold cN.
     apply sss_progress_trans with (1+eQ,v[0/pos0]).
@@ -199,7 +199,7 @@ Section mma2_simul.
   Let cN_sim : (eQ,cN) <sc (1,mma2_simul).
   Proof. unfold mma2_simul, eQ; auto. Qed.
 
-  Theorem mma2_simul_spec v : (iP,cP) // (iP,v) ↓ <-> (1,mma2_simul) // (1,v) ~~> (0,vec_zero).
+  Theorem mma2_simul_spec v : (iP,cP) //ₐ (iP,v) ↓ <-> (1,mma2_simul) //ₐ (1,v) ~~> (0,vec_zero).
   Proof.
     split.
     * intros H; apply mma_sim_spec in H; revert H.
@@ -221,5 +221,5 @@ End mma2_simul.
 (* Termination can be simulated with termination on (0,vec_zero) *)
 
 Theorem mma2_simulator i (P : list (mm_instr (pos 2))) :
-  { Q | forall v, (i,P) // (i,v) ↓ <-> (1,Q) // (1,v) ~~> (0,vec_zero) }.
+  { Q | forall v, (i,P) //ₐ (i,v) ↓ <-> (1,Q) //ₐ (1,v) ~~> (0,vec_zero) }.
 Proof. exists (mma2_simul i P); apply mma2_simul_spec. Qed.
