theories/MinskyMachines/MMA2_undec.v
@@ -13,7 +13,7 @@ From Undecidability.FRACTRAN
   Require Import FRACTRAN FRACTRAN_undec.
 
 From Undecidability.MinskyMachines 
-  Require Import MMA FRACTRAN_to_MMA2 MMA2_to_MMA2_zero.
+  Require Import MMA FRACTRAN_to_MMA2.
 
 Lemma MMA2_HALTING_undec : undecidable MMA2_HALTING.
 Proof.
@@ -25,8 +25,8 @@ Check MMA2_HALTING_undec.
 
 Lemma MMA2_HALTS_ON_ZERO_undec : undecidable MMA2_HALTS_ON_ZERO.
 Proof.
-  apply (undecidability_from_reducibility MMA2_HALTING_undec).
-  apply MMA2_MMA2_HALTS_ON_ZERO.
+  apply (undecidability_from_reducibility FRACTRAN_REG_undec).
+  apply FRACTRAN_REG_MMA2_HALTS_ON_ZERO.
 Qed.
 
 Check MMA2_HALTS_ON_ZERO_undec.
